WebAssembly/Wasm_Printing.thy
@@ -71,7 +71,17 @@ lemma[code]: "mem_rep_append (Abs_mem_rep m) n b = Abs_mem_rep (app_rev_tr (rev 
   using mem_rep_append.abs_eq
   by (simp add: append_app_rev_tr)
 
-export_code open m_imports module_type_checker interp_instantiate typing run
+(* avoid name-mangling *)
+code_identifier constant Neg \<rightharpoonup> (OCaml) "WasmRef_Isa.Neg"
+
+export_code open nat_of_byte byte_of_nat
+                 ocaml_int32_to_isabelle_int32
+                 isabelle_int32_to_ocaml_int32
+                 ocaml_int64_to_isabelle_int64
+                 isabelle_int64_to_ocaml_int64
+                 ocaml_char_to_isabelle_byte
+                 isabelle_byte_to_ocaml_char
+                 m_imports module_type_checker interp_instantiate typing run
   in OCaml module_name WasmRef_Isa file_prefix WasmRef_Isa
 
 end
